data/isabelle/src/ESPLogic/HOL_ext.thy
@@ -30,6 +30,36 @@ lemma map_leI:
   by(force simp: map_le_def)
 
 
+section{* Option *}
+
+fun opt_map2 :: "('a \<Rightarrow> 'b \<Rightarrow> 'c) \<Rightarrow> 'a option \<Rightarrow> 'b option \<Rightarrow> 'c option"
+where
+  "opt_map2 f (Some x) (Some y) = Some (f x y)"
+| "opt_map2 f _        _        = None"
+
+lemma Some_opt_map2 [simp]:
+  "(Some x = opt_map2 f a b) =
+   (\<exists> y z. x = f y z \<and> Some y = a \<and> Some z = b)"
+  "(opt_map2 f a b = Some x) =
+   (\<exists> y z. x = f y z \<and> Some y = a \<and> Some z = b)"
+  by (cases a, simp, cases b, simp_all add: eq_commute)+
+
+lemma Some_if_pushL [simp]:
+  "(Some x = (if b then Some y else None)) = (b \<and> x = y)"
+  "((if b then Some y else None) = Some x) = (b \<and> x = y)"
+  by (auto split: if_splits)
+
+lemma Some_if_pushR [simp]:
+  "(Some x = (if b then None else Some y)) = (\<not>b \<and> x = y)"
+  "((if b then None else Some y) = Some x) = (\<not>b \<and> x = y)"
+  by (auto split: if_splits)
+
+lemma Some_Option_map [simp]:
+  "(Some x = Option.map f a) = (\<exists>y. x = f y \<and> Some y = a)"
+  "(Option.map f a = Some x) = (\<exists>y. x = f y \<and> Some y = a)"
+  by (cases a, auto)+
+
+
 section{* Variadic Functions *}
 
 datatype ('a, 'b) varfun = Val 'b | Fun "'a \<Rightarrow> ('a, 'b) varfun"
